added fot maps and substitutions

fo_terms.v
@@ -7,7 +7,7 @@
 (*         CeCILL v2 FREE SOFTWARE LICENSE AGREEMENT          *)
 (**************************************************************)
 
-Require Import Extraction.
+Require Import List.
 
 Require Import acc_irr.
 
@@ -23,13 +23,46 @@ Section vec.
     | vec_nil  : vec 0
     | vec_cons : forall n, X -> vec n -> vec (S n).
 
+  Fixpoint vec2list n (v : vec n) :=
+    match v with
+      | vec_nil      => nil
+      | vec_cons x v => x::vec2list v
+    end.
+
+  Fixpoint list2vec (l : list X) : vec (length l) := 
+    match l with 
+      | nil  => vec_nil
+      | x::l => vec_cons x (list2vec l)
+    end.
+
+  Fact vec2list_length n v : length (@vec2list n v) = n.
+  Proof. induction v; simpl; f_equal; auto. Defined.
+
+  Fact list2vec_iso l : vec2list (list2vec l) = l.
+  Proof. induction l; simpl; f_equal; auto. Qed.
+
+  (* The other part needs a transport *)
+
+  Fact vec2list_iso n v : list2vec (@vec2list n v) = eq_rect_r _ v (vec2list_length v).
+  Proof. 
+    induction v; simpl; f_equal; auto.
+    rewrite IHv; unfold eq_rect_r; simpl.
+    generalize (length (vec2list v)) (vec2list_length v); intros; subst.
+    cbv; auto.
+  Qed.
+
   Variable x : X.
 
   Fixpoint in_vec n (v : vec n) : Prop :=
     match v with
       | vec_nil      => False
-      | vec_cons y v => x = y \/ in_vec v
+      | vec_cons y v => y = x \/ in_vec v
     end.
+
+  Fact in_vec_list n v : @in_vec n v <-> In x (vec2list v).
+  Proof.
+    induction v; simpl; tauto.
+  Qed.
 
 End vec.
 
@@ -62,6 +95,17 @@ Section vec_map.
                              -> @vec_in_map n v f = vec_in_map v g.
   Proof. revert f g; induction v; simpl; intros; f_equal; auto. Qed.
 
+  Fact vec_map_ext f g n v : (forall x, in_vec x v -> f x = g x) 
+                          -> @vec_map f n v = vec_map g v.
+  Proof.
+    intros H.
+    do 2 rewrite <- vec_in_map_vec_map_eq.
+    apply vec_in_map_ext, H.
+  Qed.
+
+  Fact vec2list_vec_map (f : X -> Y) n v : vec2list (@vec_map f n v) = map f (vec2list v).
+  Proof. induction v; simpl; f_equal; auto. Qed.
+
 End vec_map.
 
 Fixpoint vec_sum n (v : vec nat n) :=
@@ -74,7 +118,7 @@ Fixpoint vec_sum n (v : vec nat n) :=
 
 Section first_order_terms.
 
-  Variable (sym : Set)             (* a type of symbols *)
+  Variable (var sym : Set)         (* a type of variables and symbols *)
            (sym_ar : sym -> nat).  (* arities for symbols *)
 
   Unset Elimination Schemes.       (* we do not want the autogen recursors *)
@@ -82,6 +126,7 @@ Section first_order_terms.
   (** The Type of first order terms over signature s *)
 
   Inductive fo_term : Set :=
+    | in_var : var -> fo_term
     | in_fot : forall s, vec fo_term (sym_ar s) -> fo_term.
 
   Set Elimination Schemes.
@@ -91,38 +136,45 @@ Section first_order_terms.
     (** We build a Type level dependent recursor together with
         a fixpoint equation *)
 
-    Let sub_fo_term x t := match t with @in_fot s v => in_vec x v end.  
+    Let sub_fo_term x t := 
+      match t with 
+        | in_var _    => False 
+        | @in_fot s v => in_vec x v 
+      end.  
 
     (** This proof has to be carefully crafted for guardness *)
  
     Let Fixpoint Acc_sub_fo_term t : Acc sub_fo_term t.
     Proof.
-      destruct t as [ s v ].
-      constructor 1; simpl.
-      intros x.
-      revert v; generalize (sym_ar s).
-      induction v as [ | n y w IHw ].
-      + destruct 1.
-      + intros [ H | H ].
-        * rewrite H; apply Acc_sub_fo_term.
-        * apply IHw, H.
+      destruct t as [ x | s v ]; constructor 1; simpl.
+      + intros _ [].
+      + intros x.
+        revert v; generalize (sym_ar s).
+        induction v as [ | n y w IHw ].
+        * destruct 1.
+        * intros [ H | H ].
+          - rewrite <- H; apply Acc_sub_fo_term.
+          - apply IHw, H.
     Qed.
 
     (** This is a Type level (_rect) dependent recursor with induction
         hypothesis using Prop level in_vec *) 
 
-    Variable (P : fo_term -> Type)
+    Variable (P   : fo_term -> Type)
+             (HP0 : forall x, P (in_var x))
              (IHP : forall s v, (forall t, in_vec t v -> P t) -> P (@in_fot s v)).
 
     Let Fixpoint Fix_IHP t (Ht : Acc sub_fo_term t) { struct Ht } : P t :=
       match t as t' return Acc sub_fo_term t'-> P t' with
+        | in_var x    => fun _  => HP0 x
         | @in_fot s v => fun Ht => @IHP s v (fun x Hx => @Fix_IHP x (Acc_inv Ht _ Hx))
       end Ht.
 
     Let Fix_IHP_fix t Ht :
         @Fix_IHP t Ht 
       = match t as t' return Acc sub_fo_term t' -> _ with 
-          @in_fot s v => fun Ht' => @IHP s v (fun y H => Fix_IHP (Acc_inv Ht' H)) 
+          | in_var x    => fun _   => HP0 x
+          | @in_fot s v => fun Ht' => @IHP s v (fun y H => Fix_IHP (Acc_inv Ht' H)) 
         end Ht.
     Proof. destruct Ht; reflexivity. Qed.
 
@@ -134,7 +186,7 @@ Section first_order_terms.
     Let Fix_IHP_Acc_irr : forall t f g, @Fix_IHP t f = Fix_IHP g.
     Proof.
       apply Acc_irrelevance.
-      intros [] f g H; apply IHP_ext; auto.
+      intros [] f g H; auto; apply IHP_ext; auto.
     Qed.
 
     Theorem fo_term_rect_fix s v : 
@@ -148,22 +200,31 @@ Section first_order_terms.
 
   End fo_term_rect.
 
+  Definition fo_term_rec (P : _ -> Set) := @fo_term_rect P.
+  Definition fo_term_ind (P : _ -> Prop) := @fo_term_rect P.
+
   Section fo_term_recursion.
 
     (** We specialize the general recursor to fixed output type.
         The fixpoint equation does not require extensionality anymore *)
 
     Variable (X : Type)
-             (F : forall s, vec fo_term (sym_ar s) -> vec X (sym_ar s) -> X).
+             (F0 : var -> X)
+             (F  : forall s, vec fo_term (sym_ar s) -> vec X (sym_ar s) -> X).
 
     Definition fo_term_recursion : fo_term -> X.
     Proof.
-      induction 1 as [ s v IHv ].
-      apply (@F s v).
-      apply vec_in_map with (1 := IHv).
+      induction 1 as [ x | s v IHv ].
+      + exact (F0 x).
+      + apply (@F s v).
+        apply vec_in_map with (1 := IHv).
     Defined.
 
-    Theorem fo_term_recursion_fix s v :
+    Theorem fo_term_recursion_fix_0 x :
+      fo_term_recursion (in_var x) = F0 x.
+    Proof. reflexivity. Qed.
+
+    Theorem fo_term_recursion_fix_1 s v :
       fo_term_recursion (@in_fot s v) = F v (vec_map fo_term_recursion v).
     Proof.
       unfold fo_term_recursion at 1.
@@ -175,23 +236,144 @@ Section first_order_terms.
   End fo_term_recursion.
 
   Check fo_term_rect_fix.
-  Check fo_term_recursion_fix.
+  Check fo_term_recursion_fix_0.
+  Check fo_term_recursion_fix_1.
 
   (** We can now define eg the size of terms easily with the
       corresponding fixpoint equation *)
 
-  Definition fo_term_size : fo_term -> nat.
+  Section fo_size_dep.
+
+    Variable cost : sym -> nat.
+
+    Definition fo_term_size : fo_term -> nat.
+    Proof.
+      apply fo_term_recursion.
+      + intros _; exact 1.
+      + intros s _ v.
+        exact (cost s+vec_sum v).
+    Defined.
+
+    Fact fo_term_size_fix_0 x : 
+         fo_term_size (in_var x) = 1.
+    Proof. apply fo_term_recursion_fix_0. Qed.
+  
+    Fact fo_term_size_fix_1 s v :
+         fo_term_size (@in_fot s v) = cost s + vec_sum (vec_map fo_term_size v).
+    Proof. apply fo_term_recursion_fix_1. Qed.
+
+  End fo_size_dep.
+
+  Check fo_term_size_fix_1.
+
+  Definition fo_term_vars : fo_term -> list var.
   Proof.
     apply fo_term_recursion.
-    intros s _ v.
-    exact (1+vec_sum v).
+    + intros x; exact (x::nil).
+    + intros s _ w.
+      apply vec2list in w.
+      revert w; apply concat.
   Defined.
-  
-  Fact fo_term_size_fix s v :
-       fo_term_size (@in_fot s v) = 1 + vec_sum (vec_map fo_term_size v).
-  Proof. apply fo_term_recursion_fix. Qed.
 
-  Check fo_term_size_fix.
+  Fact fo_term_vars_fix_0 x : fo_term_vars (in_var x) = x :: nil.
+  Proof. apply fo_term_recursion_fix_0. Qed.
+
+  Fact fo_term_vars_fix_2 s v : fo_term_vars (@in_fot s v) = concat (vec2list (vec_map fo_term_vars v)).
+  Proof. apply fo_term_recursion_fix_1. Qed.
+
+  Fact fo_term_vars_fix_1 s v : fo_term_vars (@in_fot s v) = flat_map fo_term_vars (vec2list v).
+  Proof.
+    rewrite fo_term_vars_fix_2, vec2list_vec_map, <- flat_map_concat_map; auto.
+  Qed.
  
 End first_order_terms.
+
+Arguments in_var { var sym sym_ar }.
+
+Create HintDb fo_term_db.
+Tactic Notation "rew" "fot" := autorewrite with fo_term_db.
+
+Hint Rewrite fo_term_vars_fix_0 fo_term_vars_fix_1 : fo_term_db. 
+
+Section fo_term_subst.
+
+  Variable (sym : Set) (sym_ar : sym -> nat)
+           (X Y : Set).
+
+  Section subst.
+
+    Variable (f : X -> fo_term Y sym_ar).
+
+    Definition fo_term_subst : fo_term X sym_ar -> fo_term Y sym_ar.
+    Proof.
+      apply fo_term_recursion.
+      + apply f.
+      + intros s _ w; exact (in_fot s w).
+    Defined.
+
+    Fact fo_term_subst_fix_0 x : 
+         fo_term_subst (in_var x) = f x.
+    Proof. apply fo_term_recursion_fix_0. Qed.
+
+    Fact fo_term_subst_fix_1 s v : 
+         fo_term_subst (in_fot s v) = in_fot s (vec_map fo_term_subst v).
+    Proof. apply fo_term_recursion_fix_1. Qed.
+
+  End subst.
+
+  Section map.
+
+    Variable (f : X -> Y).
+
+    Definition fo_term_map : fo_term X sym_ar -> fo_term Y sym_ar.
+    Proof.
+      apply fo_term_recursion.
+      + intros x; exact (in_var (f x)).
+      + intros s _ w; exact (in_fot s w).
+    Defined.
+
+    Fact fo_term_map_fix_0 x : 
+         fo_term_map (in_var x) = in_var (f x).
+    Proof. apply fo_term_recursion_fix_0. Qed.
+
+    Fact fo_term_map_fix_1 s v : 
+         fo_term_map (in_fot s v) = in_fot s (vec_map fo_term_map v).
+    Proof. apply fo_term_recursion_fix_1. Qed.
+
+  End map.
+
+  Global Opaque fo_term_map fo_term_subst.
+
+  Global Hint Rewrite fo_term_subst_fix_0 fo_term_subst_fix_1
+               fo_term_map_fix_0 fo_term_map_fix_1 : fo_term_db.
+
+  Fact fo_term_subst_map f t : fo_term_subst (fun x => in_var (f x)) t 
+                             = fo_term_map f t.
+  Proof. induction t; rew fot; f_equal. Qed.
+
+  Fact fo_term_subst_ext f g t : (forall x, In x (fo_term_vars t) -> f x = g x)
+                               -> fo_term_subst f t = fo_term_subst g t.
+  Proof.
+    induction t as [ | s v IHv ]; intros Hfg; rew fot.
+    + apply Hfg; rew fot; simpl; auto.
+    + f_equal; apply vec_map_ext.
+      intros; apply IHv; auto.
+      intros y Hy; apply Hfg; rew fot. 
+      apply in_flat_map; exists x.
+      rewrite <- in_vec_list; tauto.
+  Qed.
+
+  Fact fo_term_map_ext f g t : (forall x, In x (fo_term_vars t) -> f x = g x)
+                             -> fo_term_map f t = fo_term_map g t.
+  Proof.
+    intros Hfg. 
+    do 2 rewrite <- fo_term_subst_map.
+    apply fo_term_subst_ext.
+    intros; f_equal; auto.
+  Qed.
+
+End fo_term_subst.
+
+
+  
 
